Propagate last_node changes to alternative spec lemmas

specs/lemmas/Spec.Blake2.Alternative.fst
@@ -15,16 +15,17 @@ module UpdateMulti = Lib.UpdateMulti
 
 val lemma_shift_update_last:
     a:alg
+  -> last_node: bool
   -> rem: nat
   -> b:block_s a
   -> d:bytes{length d + (size_block a) <= max_limb a /\ rem <= length d /\ rem <= size_block a}
   -> s:state a ->
   Lemma (
-    blake2_update_last a 0 rem (b `Seq.append` d) s ==
-    blake2_update_last a (size_block a) rem d s
+    blake2_update_last a last_node 0 rem (b `Seq.append` d) s ==
+    blake2_update_last a last_node (size_block a) rem d s
   )
 
-let lemma_shift_update_last a rem b d s =
+let lemma_shift_update_last a last_node rem b d s =
   let m = b `Seq.append` d in
   assert (Seq.slice m (length m - rem) (length m) `Seq.equal` Seq.slice d (length d - rem) (length d));
   assert (get_last_padded_block a (b `Seq.append` d) rem == get_last_padded_block a d rem)
@@ -50,14 +51,14 @@ val repeati_update1:
   -> s:state a ->
   Lemma (
     repeati nb (blake2_update1 a 0 (b `Seq.append` d)) s ==
-    repeati (nb - 1) (blake2_update1 a (size_block a) d) (blake2_update_block a false (size_block a) b s)
+    repeati (nb - 1) (blake2_update1 a (size_block a) d) (blake2_update_block a false false (size_block a) b s)
   )
 
 #push-options "--z3rlimit 100"
 let repeati_update1 a b d nb s =
   let f = blake2_update1 a 0 (b `Seq.append` d) in
   let f' = blake2_update1 a (size_block a) d in
-  let s' = blake2_update_block a false (size_block a) b s in
+  let s' = blake2_update_block a false false (size_block a) b s in
   Classical.forall_intro_2 (lemma_update1_shift a b d);
   assert (forall i s. f (i + 1) s == f' i s);
   Lems.repeati_right_shift (nb - 1) f' f s;
@@ -67,12 +68,13 @@ let repeati_update1 a b d nb s =
 
 val lemma_unfold_update_blocks:
     a:alg
+  -> last_node: bool
   -> b:block_s a
   -> d:bytes{length d > 0 /\ length d + (size_block a) <= max_limb a}
   -> s:state a ->
   Lemma (
-    blake2_update_blocks a 0 (b `Seq.append` d) s ==
-    blake2_update_blocks a (size_block a) d (blake2_update_block a false (size_block a) b s)
+    blake2_update_blocks a last_node 0 (b `Seq.append` d) s ==
+    blake2_update_blocks a last_node (size_block a) d (blake2_update_block a false false (size_block a) b s)
   )
 
 val split_one_more_block:
@@ -86,7 +88,7 @@ val split_one_more_block:
 
 let split_one_more_block a b d = ()
 
-let lemma_unfold_update_blocks a b d s =
+let lemma_unfold_update_blocks a last_node b d s =
   let nb, rem = split a (length (b `Seq.append` d)) in
   let nb', rem' = split a (length d) in
   // The condition `length d > 0` is needed for this assertion, otherwise,
@@ -94,10 +96,10 @@ let lemma_unfold_update_blocks a b d s =
   split_one_more_block a b d;
   repeati_update1 a b d nb s;
   let s_int = repeati nb (blake2_update1 a 0 (b `Seq.append` d)) s in
-  lemma_shift_update_last a rem b d s_int
+  lemma_shift_update_last a last_node rem b d s_int
 
 #push-options "--fuel 0 --ifuel 0 --z3rlimit 1000"
-let lemma_spec_equivalence_update a kk k d s =
+let lemma_spec_equivalence_update a last_node kk k d s =
   let ll = length d in
   let key_block: bytes = if kk > 0 then blake2_key_block a kk k else Seq.empty in
   if kk = 0 then begin
@@ -108,30 +110,30 @@ let lemma_spec_equivalence_update a kk k d s =
     let (nb,rem) = split a (length (blake2_key_block a kk k)) in
     // let s = repeati nb (blake2_update1 a prev (blake2_key_block a kk k)) s in
     calc (Seq.equal) {
-      blake2_update a kk k d s;
+      blake2_update a last_node kk k d s;
     (Seq.equal) {}
-      blake2_update_key a kk k ll s;
+      blake2_update_key a last_node kk k ll s;
     (Seq.equal) {}
-      blake2_update_block a true (size_block a) (blake2_key_block a kk k) s;
+      blake2_update_block a true last_node (size_block a) (blake2_key_block a kk k) s;
     (Seq.equal) { Lib.LoopCombinators.eq_repeati0 nb (blake2_update1 a 0 (blake2_key_block a kk k)) s }
-      blake2_update_blocks a 0 (blake2_key_block a kk k) s;
+      blake2_update_blocks a last_node 0 (blake2_key_block a kk k) s;
     (Seq.equal) { Seq.append_empty_r (blake2_key_block a kk k) }
-      blake2_update_blocks a 0 (blake2_key_block a kk k `Seq.append` Seq.empty) s;
+      blake2_update_blocks a last_node 0 (blake2_key_block a kk k `Seq.append` Seq.empty) s;
     (Seq.equal) { Seq.lemma_empty d }
-      blake2_update_blocks a 0 (blake2_key_block a kk k `Seq.append` d) s;
+      blake2_update_blocks a last_node 0 (blake2_key_block a kk k `Seq.append` d) s;
     (Seq.equal) { }
-      blake2_update' a kk k d s;
+      blake2_update' a last_node kk k d s;
     };
     ()
   else
     let (nb,rem) = split a (length (blake2_key_block a kk k `Seq.append` d)) in
     calc (Seq.equal) {
-      blake2_update a kk k d s;
+      blake2_update a last_node kk k d s;
     (Seq.equal) {}
-      blake2_update_blocks a (size_block a) d (blake2_update_key a kk k ll s);
+      blake2_update_blocks a last_node (size_block a) d (blake2_update_key a last_node kk k ll s);
     (Seq.equal) {}
-      blake2_update_blocks a (size_block a) d (blake2_update_block a false (size_block a) (blake2_key_block a kk k) s);
-    (Seq.equal) { lemma_unfold_update_blocks a (blake2_key_block a kk k) d s }
-      blake2_update_blocks a 0 (blake2_key_block a kk k `Seq.append` d) s;
+      blake2_update_blocks a last_node (size_block a) d (blake2_update_block a false false (size_block a) (blake2_key_block a kk k) s);
+    (Seq.equal) { lemma_unfold_update_blocks a last_node (blake2_key_block a kk k) d s }
+      blake2_update_blocks a last_node 0 (blake2_key_block a kk k `Seq.append` d) s;
     }
 #pop-options
